## 1 Pseudo-linear form

Derivation of Peyman Milanfar's gradient

$$
\begin{aligned}
\mathrm{d}[\mathbf{f}(\mathbf{x})] & =\mathrm{d}[\mathbf{A}(\mathbf{x}) \mathbf{x}] \\
& =\mathrm{d}[\mathbf{A}(\mathbf{x})] \mathbf{x}+\mathbf{A}(\mathbf{x}) \mathrm{d} \mathbf{x} \\
& =\operatorname{vec}\{\mathrm{d}[\mathbf{A}(\mathbf{x})] \mathbf{x}\}+\mathbf{A}(\mathbf{x}) \mathrm{d} \mathbf{x} \\
& =\operatorname{vec}\{\mathbf{I d}[\mathbf{A}(\mathbf{x})] \mathbf{x}\}+\mathbf{A}(\mathbf{x}) \mathrm{d} \mathbf{x} \\
& =\left(\mathbf{x}^{T} \otimes \mathbf{I}\right) \operatorname{vec}\{\mathrm{d}[\mathbf{A}(\mathbf{x})]\}+\mathbf{A}(\mathbf{x}) \mathrm{d} \mathbf{x} \\
& =\left(\mathbf{x}^{T} \otimes \mathbf{I}\right) \operatorname{Dec}[\mathbf{A}(\mathbf{x})] \mathrm{d} \mathbf{x}+\mathbf{A}(\mathbf{x}) \mathrm{d} \mathbf{x} \\
& =\left[\left(\mathbf{x}^{T} \otimes \mathbf{I}\right) \operatorname{Dec}[\mathbf{A}(\mathbf{x})]+\mathbf{A}(\mathbf{x})\right] \mathrm{d} \mathbf{x}
\end{aligned}
$$



Figure 1: Visualization of pseudo-linear gradient.
Note, a third way to derive the gradient is to use index notation:

$$
\begin{aligned}
f_{i}(\mathbf{x}) & =A_{i j}(\mathbf{x}) x_{j} \\
\Rightarrow \mathrm{~d} f_{i} & =\frac{\partial f_{i}}{\partial x_{k}} \mathrm{~d} x_{k} \\
& =\left(\frac{\partial A_{i j}}{\partial x_{k}} x_{j}+A_{i j} \delta_{j k}\right) \mathrm{d} x_{k} \\
& =\left(\frac{\partial A_{i j}}{\partial x_{k}} x_{j}+A_{i k}\right) \mathrm{d} x_{k}
\end{aligned}
$$

## 2 Chain Rule

Standard chain rule. Here we let $f \in \mathbb{R}^{d} \rightarrow \mathbb{R}$ be a scalar function, and $v \in$ $\mathbb{R}^{d} \rightarrow \mathbb{R}^{d}$ be a vector function as used in backprop.


Figure 2: Visualization of the Chain Rule: $J_{f \circ v}(x)=\nabla_{f}(v(x)) J_{v}(x)$.

## 3 Computation of the Hessian

Derivation of Yaroslav Bulatov's chain rule for the Hessian. See Figure 3.
In index notation, the Hessian of $f(v(x))$ is

$$
H_{i j}(x)=\sum_{k=1}^{d} \sum_{l=1}^{d} \frac{\partial^{2} f}{\partial u_{k} \partial u_{l}}(v(x)) \frac{\partial v_{k}}{\partial x_{i}}(x) \frac{\partial v_{l}}{\partial x_{j}}(x)+\frac{\partial f}{\partial u_{k}}(v(x)) \frac{\partial^{2} v_{k}}{\partial x_{i} \partial x_{j}}(x) .
$$

In matrix notation it is

$$
H(x)=D v(x)^{T} \cdot D^{2} f(v(x)) \cdot D v(x)+\sum_{k=1}^{d} \frac{\partial f}{\partial u_{k}}(v(x)) \frac{\partial^{2} v_{k}}{\partial x \partial x^{T}}(x)
$$

Neither of them are terribly legible.

## 4 Quadratic form

A common gradient from statistics, is the least squares $\nabla_{x}\|A x-b\|_{2}^{2}=\nabla_{x}(A x)^{T}(A x)-$ $2 b^{T} A x+b^{T} b$. See Figure 4 .

Once the gradient has been derived, we can solve for $x$ to get the usual solution $x=\left(A^{T} A\right)^{-1} A b$.

## 5 Quadratic form 2

In machine learning we sometimes want a "matrix shaped" gradient that we can easily add to the original matrix for gradient descent. Let's define a derivative notation with two edges going out for this purpose. Then we can derive the gradient with respect to $X$ of $\nabla_{X}\|X a-b\|_{2}^{2}$. See Figure 5 .


Figure 3: Visualization of the Computation of the Hessian: $H_{f \circ v}(x)=D v(x)^{T}$. $D^{2} f(v(x)) \cdot D v(x)+\sum_{k=1}^{d} \frac{\partial f}{\partial u_{k}}(v(x)) \frac{\partial^{2} v_{k}}{\partial x \partial x^{T}}(x) .$.

(x) $A-(A$

$$
\begin{gathered}
=+\mathrm{x} A-\mathrm{A}-\mathrm{x} \\
-2 \mathrm{~B} A \mathrm{x}
\end{gathered}
$$

$$
=\begin{aligned}
& 2-\mathrm{A} \\
& =-2-\mathrm{A}
\end{aligned}
$$

Figure 4: Least squares gradient, $\nabla_{x}\|A x-b\|_{2}^{2}=2 A^{T} A x-2 A b$.


$$
\begin{aligned}
& 2 a-x-x-a \\
& -2 a-x-b
\end{aligned}
$$

$$
=\quad 2 \mathrm{a}-\times(-\mathrm{a}-\mathrm{x}-\mathrm{b})
$$

Figure 5: Least squares gradient, $\nabla_{X}\|a X-b\|_{2}^{2}=2 a \otimes(X a-b)$. In step four we used a small trick, which is that $x^{T}(I \otimes I) x=(I \otimes I)(x \otimes x)=(I x) \otimes(I x)=x \otimes x$. In other words, the degree 4 identity matrix splits into the outer product of it's constituents.

